StructuredEncryption/test/Paths.dfy
@@ -1,6 +1,7 @@
 // Copyright Amazon.com Inc. or its affiliates. All Rights Reserved.
 // SPDX-License-Identifier: Apache-2.0
 include "../src/Paths.dfy"
+include "../src/Virtual.dfy"
 
 module PathsTests {
   import opened Wrappers
@@ -8,105 +9,7 @@ module PathsTests {
   import opened StandardLibrary.UInt
   import opened StructuredEncryptionUtil
   import opened StructuredEncryptionPaths
-
-  // This first part converts strings to TerminalLocations
-  // It will be moved to src/Paths when we do Beacons 
-
-  // return the number of characters until the next part begins
-  // that is, '[' or '.'
-  function method  {:opaque} FindStartOfNext(s : string)
-    : (index : Option<nat>)
-    ensures index.Some? ==> 
-      && index.value < |s|
-      && (s[index.value] == '.' || s[index.value] == '[')
-      && '.' !in s[..index.value]
-      && '[' !in s[..index.value]
-    ensures index.None? ==> '.' !in s && '[' !in s
-  {
-    var dot := FindIndexMatching(s, '.', 0);
-    var bracket := FindIndexMatching(s, '[', 0);
-    if dot.None? && bracket.None? then
-      None
-    else if dot.Some? && bracket.Some? then
-      if dot.value < bracket.value then
-        dot
-      else
-        bracket
-    else if dot.Some? then
-      dot
-    else
-      bracket
-  }
-
-  // read an unsigned decomal number, return value and length
-  function method {:tailrecursion} {:opaque} GetNumber(s : string, acc : nat := 0)
-    : Result<nat, string>
-  {
-    if |s| == 0 then
-      Success(acc)
-    else if '0' <= s[0] <= '9' then
-      GetNumber(s[1..], acc * 10 + s[0] as nat - '0' as nat)
-    else
-      Failure("Unexpected character in number : " + [s[0]])
-  }
-
-  // make Map from string
-  function method  {:opaque} MakeMap(s : string) : (ret : Result<Selector, string>)
-    ensures ret.Success? ==> ret.value.Map?
-  {
-    :- Need(ValidString(s), "Key string invalid.");
-    Success(Map(s))
-  }
-
-  // convert string to Selector
-  function method {:opaque} GetSelector(s : string)
-    : Result<Selector, string>
-    requires |s| > 0 && (s[0] == '.' || s[0] == '[')
-  {
-    if s[0] == '.' then
-      var m :- MakeMap(s[1..]);
-      Success(m)
-    else
-      if s[|s|-1] != ']' then
-        Failure("List index must end with ]")
-      else
-        var num :- GetNumber(s[1..|s|-1]);
-        :- Need(num < UINT64_LIMIT, "Array selector exceeds maximum.");
-        Success(List(num as uint64))
-  }
-
-  // convert string to SelectorList
-  function method {:tailrecusrion} {:opaque} GetSelectors(s : string, acc : SelectorList := [])
-    : Result<SelectorList, string>
-    requires |s| > 0 && (s[0] == '.' || s[0] == '[')
-  {
-    var pos := FindStartOfNext(s[1..]);
-    var end := if pos.None? then |s| else pos.value + 1;
-    var sel : Selector :- GetSelector(s[..end]);
-    :- Need(|acc|+1 < UINT64_LIMIT, "Selector Overflow");
-    if pos.None? then
-      Success(acc + [sel])
-    else
-      GetSelectors(s[end..], acc + [sel])
-  }
-
-  // convert string to TerminalLocation
-  function method {:opaque} MakeTerminalLocation(s : string)
-    : (ret : Result<TerminalLocation, string>)
-    ensures ret.Success? ==> 0 < |ret.value.parts|
-  {
-    :- Need(0 < |s|, "Path specification must not be empty.");
-    var pos := FindStartOfNext(s);
-    if pos.None? then
-      var m :- MakeMap(s);
-      Success(TerminalLocation([m]))
-    else
-      var name := s[..pos.value];
-      var selectors :- GetSelectors(s[pos.value..]);
-      var m :- MakeMap(name);
-      :- Need(|selectors|+1 < UINT64_LIMIT, "Selector Overflow");
-      Success(TerminalLocation([m] + selectors))
-  }
+  import opened VirtualFields
 
   method {:test} TestSpecExamples() {
     var tableName : GoodString := "example_table";
