DynamoDbItemEncryptor/src/VirtualDDB.dfy
@@ -1,0 +1,118 @@
+// Copyright Amazon.com Inc. or its affiliates. All Rights Reserved.
+// SPDX-License-Identifier: Apache-2.0
+
+/*
+  The entry points of interest are
+
+  // Stringify a TerminalLocation in the context of an AttributeMap
+  TermToString(t : TerminalLocation, item : DDB.AttributeMap) : string
+
+  This is generally used this way
+  VirtualField f = GetVirtualField(spec);
+  fieldValue := f.makeString(t => TermToString(t, item));
+
+  // calculate all virtual field values, in the same way as PutItem et al
+  GetVirtualAttributes(fields : seq<VirtualField>, item : DDB.AttributeMap) : DDB.AttributeMap
+*/
+
+include "../Model/AwsCryptographyDynamoDbItemEncryptorTypes.dfy"
+include "../../StructuredEncryption/src/Virtual.dfy"
+
+module VirtualDDBFields {
+  import opened StandardLibrary
+  import opened Wrappers
+  import DDB = ComAmazonawsDynamodbTypes
+  import Base64
+  import opened StandardLibrary.UInt
+  import opened StructuredEncryptionUtil
+  import opened StructuredEncryptionPaths
+  import opened VirtualFields
+
+  // return true if item does not have the given terminal
+  predicate method LacksAttribute(t : TerminalLocation, item : DDB.AttributeMap)
+  {
+    t.parts[0].key !in item
+  }
+
+  // return true if item has all of the terminals necessary for field
+  predicate method ValueHasNeededAttrs(field : VirtualField, item : DDB.AttributeMap)
+  {
+    !field.examine(t => LacksAttribute(t, item))
+  }
+
+  // return the string value for the given terminal in the given item
+  function method TermToString(t : TerminalLocation, item : DDB.AttributeMap)
+    : Result<string,string>
+  {
+    if t.parts[0].key !in item then
+      Failure("Requested attribute " + t.parts[0].key + " not in item.")
+    else
+      AttrValueToString(item[t.parts[0].key], t.parts[1..])
+  }
+
+  // return the string value for the given terminal in the given value
+  function method {:tailrecursion} {:opaque} AttrValueToString(v : DDB.AttributeValue, parts : seq<Selector>)
+    : Result<string, string>
+  {
+    match v {
+      case S(s) => NeedEmpty(s, parts)
+      case N(s) => NeedEmpty(s, parts)
+      case B(b) => NeedEmpty(Base64.Encode(b), parts)
+      case SS(s) => Failure("Can't do sets")
+      case NS(s) => Failure("Can't do sets")
+      case BS(s) => Failure("Can't do sets")
+      case BOOL(b) => NeedEmpty(if b then "true" else "false", parts)
+      case NULL(n) => NeedEmpty("null", parts)
+      case L(l) =>
+        if |parts| == 0 then
+          Failure("Tried to access list without parts.")
+        else if !parts[0].List? then
+          Failure("Tried to access list with key")
+        else if |l| <= parts[0].pos as int then
+          Failure("Tried to access beyond the end of the list")
+        else
+          AttrValueToString(l[parts[0].pos], parts[1..])
+      case M(m) =>
+        if |parts| == 0 then
+          Failure("Tried to access map without parts.")
+        else if !parts[0].Map? then
+          Failure("Tried to access map with index")
+        else if parts[0].key !in m then
+          Failure("Tried to access " + parts[0].key + " which is not in the map.")
+        else
+          AttrValueToString(m[parts[0].key], parts[1..])
+    }
+  }
+
+  // return true if everything in the AttributeMap is of type string
+  predicate AllStrings(item : DDB.AttributeMap) {
+    forall x <- item :: item[x].S?
+  }
+
+  // convert string to DynamoDB Attribute
+  function method DS(s : string)
+    : DDB.AttributeValue
+  {
+    DDB.AttributeValue.S(s)
+  }
+
+  // return an AttributeMap containing all of the virtual fields for which we have the appropriate attributes
+  function method {:tailrecursion} GetVirtualAttrs (
+    fields : seq<VirtualField>,
+    item : DDB.AttributeMap,
+    acc : DDB.AttributeMap := map[])
+    : (ret : Result<DDB.AttributeMap, string>)
+    requires AllStrings(acc)
+    ensures ret.Success? ==> AllStrings(ret.value)
+  {
+    if |fields| == 0 then
+      Success(acc)
+    else
+      :- Need(DDB.IsValid_AttributeName(fields[0].name), "Virtual field name '" + fields[0].name + "' is not a valid DynamoDB Attribute Name");
+      if ValueHasNeededAttrs(fields[0], item) then
+        var value :- fields[0].makeString(t => TermToString(t, item));
+        GetVirtualAttrs(fields[1..], item, acc[fields[0].name := DDB.AttributeValue.S(value)])
+      else
+        GetVirtualAttrs(fields[1..], item, acc)
+  }
+}
