DynamoDbItemEncryptor/test/VirtualDDB.dfy
@@ -1,0 +1,58 @@
+include "../src/VirtualDDB.dfy"
+
+module VirtualDDBFieldsTests {
+  import opened Wrappers
+  import opened StandardLibrary
+  import opened StandardLibrary.UInt
+  import opened StructuredEncryptionUtil
+  import opened StructuredEncryptionPaths
+  import opened VirtualFields
+  import opened VirtualDDBFields
+  import DDB = ComAmazonawsDynamodbTypes
+
+  method CheckValueString(expr : string, data : DDB.AttributeMap, expected : string) {
+    var val := VirtualFields.GetVirtualField("foo", expr);
+    var val2 :- expect val;
+    if !ValidVirtualField(val2) {
+      print "Invalid Value : ", val2, "\n";
+    }
+    expect ValidVirtualField(val2);
+
+    var str := val2.makeString(t => TermToString(t, data));
+    var actual :- expect str;
+
+    if actual != expected {
+      print "Expected ", expected, " actual ", actual, "\n";
+    }
+    expect actual == expected;
+  }
+
+  method {:test} TestMakeString() {
+    var data : DDB.AttributeMap := map["attr" := DS("12345"), "other" := DS("abcde"), "third" := DS("a.b.c.d.e")];
+    CheckValueString("attr + other", data, "12345abcde");
+    CheckValueString("attr | Prefix 3 + other | Suffix 3", data, "123cde");
+    CheckValueString("attr + third | Parts . 3 4", data, "12345c.d");
+    CheckValueString("attr + Literal _ + third | Parts . 3 4", data, "12345_c.d");
+    CheckValueString("attr + Literal _ + third | Parts . 3", data, "12345_c");
+  }
+  method {:test} TestMakeString2() {
+    var data : DDB.AttributeMap := map[
+      "bool" := DDB.AttributeValue.BOOL(true),
+      "null" := DDB.AttributeValue.NULL(true),
+      "number" := DDB.AttributeValue.N("123"),
+      "binary" := DDB.AttributeValue.B([1,2,3]),
+      "list" := DDB.AttributeValue.L([
+        DS("abc"),
+        DS("def"),
+        DS("ghi")
+      ]),
+      "map" := DDB.AttributeValue.M(map[
+        "key1" := DS("jkl"),
+        "key2" := DS("mno"),
+        "key3" := DS("pqr")
+      ])
+    ];
+    CheckValueString("list[1] + map.key2", data, "defmno");
+    CheckValueString("bool + null + number + binary", data, "truenull123AQID");
+  }
+}
