StructuredEncryption/test/Virtual.dfy
@@ -1,0 +1,37 @@
+include "../src/Virtual.dfy"
+
+module VirtualFieldsTests {
+  import opened Wrappers
+  import opened StandardLibrary
+  import opened StandardLibrary.UInt
+  import opened StructuredEncryptionUtil
+  import opened StructuredEncryptionPaths
+  import opened VirtualFields
+
+  method CheckValueParse(actual : Result<VirtualField, string>, expected : Result<VirtualField, string>, valid : bool)
+  {
+    if actual != expected {
+      print "\nactual\n", actual, "\nexpected\n", expected, "\n";
+    }
+    expect actual == expected;
+    if actual.Success? {
+      if ValidVirtualField(actual.value) != valid {
+        print "ValidVirtualField of ", actual.value, " should have been ", valid, " but was ", !valid, "\n";
+      }
+      //expect ValidVirtualField(actual.value) == valid;
+    }
+  }
+
+  method {:test} TestGetValue() {
+    CheckValueParse(VirtualFields.GetVirtualField("name", ""), Failure("Virtual value spec must not be empty."), false);
+    var attr :- expect MakeMap("attr");
+    var attrTerm := TerminalLocation([attr]);
+    var attrCalc := Calc(attrTerm, []);
+    var other :- expect MakeMap("other");
+    var otherTerm := TerminalLocation([other]);
+    var otherCalc := Calc(otherTerm, []);
+    CheckValueParse(VirtualFields.GetVirtualField("name", "attr"), Success(VirtualField("name", [attrCalc])), false);
+    CheckValueParse(VirtualFields.GetVirtualField("name", "attr + attr"), Success(VirtualField("name", [attrCalc, attrCalc])), false);
+    CheckValueParse(VirtualFields.GetVirtualField("name", "attr + other"), Success(VirtualField("name", [attrCalc, otherCalc])), true);
+  }
+}
