specification/structured-encryption/virtual-field.md
@@ -1,0 +1,171 @@
+[//]: # "Copyright Amazon.com Inc. or its affiliates. All Rights Reserved."
+[//]: # "SPDX-License-Identifier: CC-BY-SA-4.0"
+
+# Virtual Fields
+
+## Version
+
+1.0.0
+
+### Changelog
+
+## Overview
+
+A virtual field is a field constructed from parts of other fields, but never stored in the database.
+
+A virtual field can be used in the construction of a [compound beacon](beacons.md#compound-beacon)
+which can be stored in the database and can be used to search.
+
+A virtual field is configured by specifying [terminal locations](#terminal location),
+[modifying](#field-modifications), and combining them with [literal values](#literal-value).
+
+If an encrypted field is involved in the construction of a virtual field,
+then the virtual field can only be used in a [sensitive part](beacons.md#sensitive-part).
+
+For example imagine this fraction of a database record :
+```
+{
+  FirstName : "John",
+  FamilyName : {
+    LastNames : [
+      "Smith",
+      "Jones"
+    ]
+  }
+}
+```
+
+If one wanted to be able to search on a `NameTag` field that had the value `jsmith`,
+one specify `NameTag` to be a virtual field with this configuration :
+
+`FirstName | Prefix 1 | Lower + FamilyName.LastNames[0] | Lower`
+
+If a customer then configured a [standard beacon](#beacons.md#standard-beacon)
+on the `NameTag` field, they would then query on
+`NameTag = jsmith` and the right record would be retrieved.
+
+The customer is responsible for generating the text "jsmith" at query time.
+
+One of the primary customer benefits is that this allows a beacon on a sub-part
+of a structured value.
+
+### Terminal Location
+
+A Terminal Location specifies the location of a piece of data within a structure.
+In the example above `FirstName` and `FamilyName.LastNames[0]` are examples of
+terminal locations. At the moment, a terminal locations must resolve to a string
+(i.e. not a map, list or set) but this might be relaxed in future versions.
+
+A terminal location MUST be a field name followed by zero or more [Segments](#segments)
+
+#### Segments
+
+A Segment MUST be one of
+
+ - A literal "." followed by a field name, indicating a lookup into a Structured Data Map.
+ - A literal "[" followed by a decimal integer followed by a literal "]",
+indicating an index into a  Structured Data List.
+
+### Field Modifications
+
+The following functions MUST be provided to modify strings
+
+* "Prefix" N - the first N characters (not bytes). The unmodified string if N > length.
+* "Suffix" N - the last N characters (not bytes). The unmodified string if N > length.
+* "Lower" - any ascii letters replaced with their lowercase equivalent.
+* "Upper" - any ascii letters replaced with their uppercase equivalent.
+* "Parts" Char Low High - Split the string on Char, keep only the parts Low..High inclusive.
+Both Low and High reduced to total parts. High is optional, and defaults to Low.
+
+### Virtual Segment
+
+A virtual segment MUST be one of
+ - a [literal value](#literal-value)
+ - a [value calculation](#value-calculation)
+
+#### Literal Value
+
+A literal value must be the string "Literal" followed by whitespace followed by
+a string that contains no whitespace.
+
+#### Value Calculation
+
+A value calculation MUST be a [terminal location](#terminal-location) followed by zero or more
+" | " delimited Field Modifications.
+
+For example, `FirstName | Lower | Prefix 1`
+
+ 1 [Stringifys](#stringify) the FirstName field
+ 1 Converts it to lowercase
+ 1 Discards all but the first character
+
+### Virtual Field Definition
+
+A virtual value is " + " delimited list of [virtual segments](#virtual-segement).
+
+For example the NameTag example above might be specified as
+
+`FirstName | Prefix 1 | Lower + FamilyName.LastNames[0] | Lower`
+
+Or the full name, with an underscore between the first and last name, would be
+
+`FirstName | Lower + Literal _ + FamilyName.LastNames[0] | Lower`
+
+#### GetVirtualField
+
+The function GetVirtualField MUST be provided, taking a name and a [virtual field definition](#virtual-field-definition) and returning a VirtualField.
+
+### Stringify
+
+A virtual field is always a string, and so all [terminal locations](#terminal-location)
+must be converted to strings before being used to construct a virtual field.
+
+Stringify MUST be a a callback function that takes a Terminal Location and returns a string.
+
+This callback is NOT accessible to the customer, but is simply a bridge between the
+structured encryption layer and the database layer.
+
+For example, a DynamoDB callback might resolve a Path on an ItemMap and produce
+a string based on the type of the Terminal.
+
+####  VirtualField.makeString
+
+A VirtualField MUST provide the method makeString,
+which takes a [Stringify](#stringify) and returns a string.
+
+makeString MUST calculate the virtual field as defined above,
+translating [terminal locations](#terminal-location) into strings
+with the provided [Stringify](#stringify).
+
+### Examiner
+
+It can be important to know if a virtual field has a certain quality,
+defined as any of its parts having the quality.
+
+Examiner MUST be a a callback function that takes a Terminal Location and returns a boolean.
+
+For example, an DynamoDB callback might check to see if the top level 
+field is encrypted or signed.
+
+#### VirtualField.examine
+
+A VirtualField MUST provide the method examine,
+which takes a [Examiner](#examiner) and returns a boolean.
+
+examine MUST return `true` if the [Examiner](#examiner) returns `true`
+for any [terminal locations](#terminal-location)] in the virtual field,
+and `false` otherwise.
+
+### Limitations
+
+It is an error to write an field with the same name as a
+[virtual field](#virtual-field-configuration).
+
+If you write an item with a given field, and later define a virtual field
+with that same name, then future searches will search only on the virtual field,
+and you will not be able to find the item base on the original field value.
+
+Because of the syntax above
+
+* The ` + ` and ` | ` that delimit pieces must be surrounded by whitespace
+* Literal Values and field names cannot contain whitespace.
